theories/Mem1.v
@@ -87,7 +87,7 @@ Section PROOF.
 
   Definition mem: ModSem.t := {|
     ModSem.fnsems := [("alloc", allocF) ; ("free", freeF)];
-    ModSem.initial_mrs := [("mem", GRA.padding (URA.black (M:=_memRA) (inr tt)))];
+    ModSem.initial_mrs := [("mem", GRA.padding (URA.black (M:=_memRA) (inl (fun _ _ => None))))];
   |}
   .
 End PROOF.
